Hashmap/DHashMap/Index.lean
@@ -5,6 +5,7 @@ Authors: Markus Himmel
 -/
 import Hashmap.PowerOfTwo
 import Std.Data.UInt
+import Hashmap.LawfulHashable
 
 -- This file needs a lot of clean-up, but I don't really want to get bogged down with this too much at the moment
 
@@ -34,64 +35,90 @@ theorem USize.toNat_sub_le {a b : Nat} (h : b ≤ a) : a.toUSize - b.toUSize = (
 
 theorem Nat.toUSize_one : (1 : Nat).toUSize = 1 := rfl
 
--- An array size is good if it is a small power of two, so that index arithmetic can be performed as bit arithmetic on small numbers.
--- This is also better than just the power-of-two requirement because it ensures that the checkSize method is total.
-structure IsGoodSize (sz : Nat) : Prop where
-  isPowerOfTwo : sz.isPowerOfTwo
-  lt : sz < USize.size
+theorem USize.toNat_lt' {a : USize} : a.toNat < USize.size :=
+  a.1.2
 
-theorem isGoodSize_iff {sz : Nat} : IsGoodSize sz ↔ 0 < sz ∧ sz < USize.size ∧ (sz.toUSize &&& (sz.toUSize - 1)) = 0 := by
-  refine ⟨?_, ?_⟩
-  · rintro ⟨h₁, h₂⟩
-    refine ⟨Nat.pos_of_isPowerOfTwo h₁, h₂, ?_⟩
-    rw [isPowerOfTwo_iff] at h₁
-    apply USize.ext
-    rw [USize.toNat_and, Nat.toNat_toUSize h₂, ← Nat.toUSize_one, USize.toNat_sub_le h₁.1, USize.zero_toNat, Nat.toNat_toUSize]
-    · exact h₁.2
-    · exact Nat.lt_of_le_of_lt (Nat.sub_le _ _) h₂
-  · rintro ⟨h₁, h₂, h₃⟩
-    refine ⟨?_, h₂⟩
-    rw [isPowerOfTwo_iff]
-    refine ⟨h₁, ?_⟩
-    have := congrArg USize.toNat h₃
-    rw [USize.toNat_and, Nat.toNat_toUSize h₂, ← Nat.toUSize_one, USize.toNat_sub_le h₁, USize.zero_toNat, Nat.toNat_toUSize] at this
-    · exact this
-    · exact Nat.lt_of_le_of_lt (Nat.sub_le _ _) h₂
+-- structure IsGoodSize (sz : Nat) : Prop where
+--   pos : 0 < sz
+--   lt : sz < USize.size
 
-@[inline] def checkSize (sz : Nat) : Bool :=
-  decide (0 < sz ∧ sz < USize.size ∧ (sz.toUSize &&& (sz.toUSize - 1)) = 0)
+-- theorem isGoodSize_iff {sz : Nat} : IsGoodSize sz ↔ 0 < sz ∧ sz < USize.size ∧ (sz.toUSize &&& (sz.toUSize - 1)) = 0 := by
+--   refine ⟨?_, ?_⟩
+--   · rintro ⟨h₁, h₂⟩
+--     refine ⟨Nat.pos_of_isPowerOfTwo h₁, h₂, ?_⟩
+--     rw [isPowerOfTwo_iff] at h₁
+--     apply USize.ext
+--     rw [USize.toNat_and, Nat.toNat_toUSize h₂, ← Nat.toUSize_one, USize.toNat_sub_le h₁.1, USize.zero_toNat, Nat.toNat_toUSize]
+--     · exact h₁.2
+--     · exact Nat.lt_of_le_of_lt (Nat.sub_le _ _) h₂
+--   · rintro ⟨h₁, h₂, h₃⟩
+--     refine ⟨?_, h₂⟩
+--     rw [isPowerOfTwo_iff]
+--     refine ⟨h₁, ?_⟩
+--     have := congrArg USize.toNat h₃
+--     rw [USize.toNat_and, Nat.toNat_toUSize h₂, ← Nat.toUSize_one, USize.toNat_sub_le h₁, USize.zero_toNat, Nat.toNat_toUSize] at this
+--     · exact this
+--     · exact Nat.lt_of_le_of_lt (Nat.sub_le _ _) h₂
 
-theorem checkSize_eq_true {sz : Nat} : checkSize sz = true ↔ IsGoodSize sz := by
-  simp [isGoodSize_iff, checkSize]
+-- @[inline] def checkSize (sz : Nat) : Bool :=
+--   decide (0 < sz ∧ sz < USize.size)
+
+-- theorem checkSize_eq_true {sz : Nat} : checkSize sz = true ↔ IsGoodSize sz := by
+--   simp [checkSize]; exact ⟨fun ⟨h₁, h₂⟩ => ⟨h₁, h₂⟩, fun ⟨h₁, h₂⟩ => ⟨h₁, h₂⟩⟩
 
 -- Double the size if it is not already huge
-def nextSize (sz : { sz : Nat // IsGoodSize sz }) : { sz : Nat // IsGoodSize sz } :=
-  let ⟨n, ⟨h₁, h₂⟩⟩ := sz
-  if h : n * 2 < USize.size then
-    ⟨n * 2, ⟨Nat.mul2_isPowerOfTwo_of_isPowerOfTwo h₁, h⟩⟩
-  else
-    ⟨n, ⟨h₁, h₂⟩⟩
+-- def nextSize (sz : { sz : Nat // IsGoodSize sz }) : { sz : Nat // IsGoodSize sz } :=
+--   let ⟨n, ⟨h₁, h₂⟩⟩ := sz
+--   if h : n * 2 < USize.size then
+--     ⟨n * 2, ⟨Nat.mul_pos h₁ Nat.two_pos, h⟩⟩
+--   else
+--     ⟨n, ⟨h₁, h₂⟩⟩
 
 -- TODO: benchmark if we need a C implementation for this. Currently this still needs to do a scalar check for sz which we could
 -- maybe get rid of, if we changed to size condition in IsGoodSize to assert that sz is definitely a scalar.
-def mkIdx {sz : Nat} (hash : UInt64) (h : IsGoodSize sz) : { u : USize // u.toNat < sz } :=
+-- Note that this indexing scheme always produces a valid index, but it has a chance of returning every index if sz is a power of two.
+def mkIdx {sz : Nat} (hash : UInt64) (h : 0 < sz) : { u : USize // u.toNat < sz } :=
   ⟨hash.toUSize &&& (sz.toUSize - 1), by
-    rw [USize.toNat_and, ← Nat.toUSize_one, USize.toNat_sub_le, Nat.toNat_toUSize]
-    · obtain ⟨k, rfl⟩ := h.isPowerOfTwo
-      simpa using Nat.mod_lt _ (Nat.pow_pos Nat.two_pos)
-    · have := h.lt
-      omega
-    · exact Nat.pos_of_isPowerOfTwo h.isPowerOfTwo⟩
+    by_cases h' : sz < USize.size
+    · rw [USize.toNat_and, ← Nat.toUSize_one, USize.toNat_sub_le, Nat.toNat_toUSize]
+      · refine Nat.lt_of_le_of_lt and_le_right ?_
+        exact Nat.sub_lt h Nat.one_pos
+      · exact Nat.lt_of_le_of_lt (Nat.sub_le _ _) h'
+      · exact h
+    · exact Nat.lt_of_lt_of_le USize.toNat_lt' (Nat.le_of_not_lt h')⟩
+
+-- @[simp]
+-- theorem mkIdx_val {sz : Nat} {hash : UInt64} {h : IsGoodSize sz} : (mkIdx hash h).val = hash.toUSize % sz := by
+--   rw [mkIdx]
+--   simp
+--   apply USize.ext
+--   rw [USize.toNat_and, ← Nat.toUSize_one, USize.toNat_sub_le, Nat.toNat_toUSize]
+--   · obtain ⟨k, rfl⟩ := h.isPowerOfTwo
+--     simp
+--     erw [USize.modn_toNat]
+--   · have := h.lt
+--     omega
+--   · exact Nat.pos_of_isPowerOfTwo h.isPowerOfTwo
+
+namespace List
+
+variable {α : Type u} {β : α → Type v}
+
+structure HashesTo [BEq α] [Hashable α] (l : List (Σ a, β a)) (i : Nat) (size : Nat) : Prop where
+  hash_self : (h : 0 < size) → ∀ p, p ∈ l → (mkIdx (hash p.1) h).1.toNat = i
 
 @[simp]
-theorem mkIdx_val {sz : Nat} {hash : UInt64} {h : IsGoodSize sz} : (mkIdx hash h).val = hash.toUSize % sz := by
-  rw [mkIdx]
-  simp
-  apply USize.ext
-  rw [USize.toNat_and, ← Nat.toUSize_one, USize.toNat_sub_le, Nat.toNat_toUSize]
-  · obtain ⟨k, rfl⟩ := h.isPowerOfTwo
-    simp
-    erw [USize.modn_toNat]
-  · have := h.lt
-    omega
-  · exact Nat.pos_of_isPowerOfTwo h.isPowerOfTwo
+theorem hashesTo_nil [BEq α] [Hashable α] {i : Nat} {size : Nat} :
+    ([] : List (Σ a, β a)).HashesTo i size where
+  hash_self := by simp
+
+theorem hashesTo_cons [BEq α] [Hashable α] [LawfulHashable α] {i : Nat} {size : Nat} {l : List (Σ a, β a)} {k : α}
+    {v : β k} (h : (h' : 0 < size) → (mkIdx (hash k) h').1.toNat = i) :
+    l.HashesTo i size → (⟨k, v⟩ :: l).HashesTo i size := by
+  refine fun ⟨ih⟩ => ⟨fun h' k' hk => ?_⟩
+  simp only [mem_cons] at hk
+  rcases hk with (rfl|hk)
+  · exact h h'
+  · exact ih h' _ hk
+
+end List
