Hashmap/DHashMap/Lemmas.lean
@@ -65,7 +65,8 @@ theorem exists_bucket_of_uset [BEq α] [Hashable α]
     ∃ l, self.data.bind AssocList.toList ~ self[i.toNat].toList ++ l ∧
       (self.uset i d hi).data.bind AssocList.toList ~ d.toList ++ l ∧
       (∀ [EquivBEq α] [LawfulHashable α],
-        IsHashSelf self → ∀ k : α, ((hash k).toUSize % self.size).toNat = i.toNat → l.containsKey k = false) := by
+        IsHashSelf self → ∀ k : α, (mkIdx (hash k) (show 0 < self.size by omega)).1.toNat = i.toNat → l.containsKey k = false) := by
+  have h₀ : 0 < self.size := by omega
   obtain ⟨l₁, l₂, h₁, h₂, h₃⟩ := Array.exists_of_update self i d hi
   refine ⟨l₁.bind AssocList.toList ++ l₂.bind AssocList.toList, ?_, ?_, ?_⟩
   · rw [h₁]
@@ -79,16 +80,17 @@ theorem exists_bucket_of_uset [BEq α] [Hashable α]
     obtain ⟨⟨k', v'⟩, ⟨(⟨a, ha₁, ha₂⟩|⟨a, ha₁, ha₂⟩), hk⟩⟩ := hk
     · obtain ⟨n, hn⟩ := List.get_of_mem ha₁
       rw [List.get_eq_get_append_right (self[i] :: l₂)] at hn
-      suffices ((hash k').toUSize % self.size).toNat = n from
+      suffices (mkIdx (hash k') h₀).1.toNat = n from
         Nat.ne_of_lt (Nat.lt_of_eq_of_lt (hash_eq hk ▸ this) (h₂ ▸ n.2))
       rw [List.get_congr h₁.symm, ← Array.getElem_eq_data_get] at hn
-      exact (h.hashes_to n (by omega)).hash_self _ (hn.symm ▸ ha₂)
+      exact (h.hashes_to n (by omega)).hash_self h₀ _ (hn.symm ▸ ha₂)
     · obtain ⟨n, hn⟩ := List.get_of_mem ha₁
       rw [List.get_eq_get_cons self[i], List.get_eq_get_append_left l₁] at hn
-      suffices ((hash k').toUSize % self.size).toNat = n + 1 + l₁.length from
-        Nat.ne_of_lt' (h₂ ▸ ((hash_eq hk ▸ this) ▸ by omega))
+      suffices (mkIdx (hash k') h₀).1.toNat = n + 1 + l₁.length by
+        refine Nat.ne_of_lt' ?_
+        simp only [← hash_eq hk, this, h₂, Nat.lt_add_left_iff_pos, Nat.succ_pos]
       rw [List.get_congr h₁.symm, ← Array.getElem_eq_data_get] at hn
-      refine (h.hashes_to (n + 1 + l₁.length) ?_).hash_self _ (hn.symm ▸ ha₂)
+      refine (h.hashes_to (n + 1 + l₁.length) ?_).hash_self h₀ _ (hn.symm ▸ ha₂)
       rw [Array.size_eq_length_data, h₁, length_append, length_cons]
       omega
 
@@ -96,38 +98,30 @@ theorem exists_bucket [BEq α] [Hashable α]
     (self : Array (AssocList α β)) (i : USize) (hi : i.toNat < self.size) :
       ∃ l, self.data.bind AssocList.toList ~ self[i.toNat].toList ++ l ∧
         (∀ [EquivBEq α] [LawfulHashable α], IsHashSelf self → ∀ k,
-          ((hash k).toUSize % self.size).toNat = i.toNat → l.containsKey k = false) := by
+          (mkIdx (hash k) (show 0 < self.size by omega)).1.toNat = i.toNat → l.containsKey k = false) := by
   obtain ⟨l, h₁, -, h₂⟩ := exists_bucket_of_uset self i hi .nil
   exact ⟨l, h₁, h₂⟩
 
 namespace Raw
 
-theorem empty_eq (c) : ∃ c', (empty c : Raw α β) = ⟨0, mkArray c' AssocList.nil⟩ := by
-  dsimp [empty]
-  split <;> exact ⟨_, rfl⟩
-
 @[simp]
-theorem size_empty {c} : (empty c : Raw α β).size = 0 := by
-  obtain ⟨c', h⟩ := empty_eq c
-  rw [h]
+theorem size_empty {c} : (empty c : Raw α β).size = 0 := rfl
 
 @[simp]
 theorem toList_empty {c} : (empty c : Raw α β).toList = [] := by
-  suffices ∀ d, (List.replicate d AssocList.nil).bind AssocList.toList = [] by
-    obtain ⟨c', h⟩ := empty_eq c
-    exact h ▸ this _
+  suffices ∀ d, (List.replicate d AssocList.nil).bind AssocList.toList = [] from this _
   intro d
   induction d <;> simp_all
 
 theorem findEntry?WellFormed_eq_findEntry_toList [BEq α] [EquivBEq α] [Hashable α] [LawfulHashable α]
-    (m : { m : Raw α β // IsGoodSize m.buckets.size }) (h : m.1.ActuallyWF) (a : α) :
+    (m : { m : Raw α β // 0 < m.buckets.size }) (h : m.1.ActuallyWF) (a : α) :
       Raw.findEntry?WellFormed m a = m.1.toList.findEntry? a := by
   rw [findEntry?WellFormed]
   dsimp only [Array.ugetElem_eq_getElem]
   obtain ⟨l, hl, hlk⟩ := exists_bucket m.1.buckets (mkIdx (hash a) m.2).1 (mkIdx (hash a) m.2).2
   refine Eq.trans ?_ (List.findEntry?_of_perm (WF_of_perm hl.symm h.distinct) hl.symm)
   rw [AssocList.findEntry?_eq, findEntry?_append_of_containsKey_eq_false]
-  exact hlk h.buckets_hash_self _ (by simp only [mkIdx_val])
+  refine hlk h.buckets_hash_self _ rfl
 
 end Raw
 
